Hw8 submitted.

sf/Assignment08_05.v
@@ -7,7 +7,13 @@ Require Export Assignment08_04.
     same as pushing the value of the expression on the stack. *)
 
 Fixpoint s_compile (e : aexp) : list sinstr :=
-  FILL_IN_HERE.
+match e with
+ | ANum v => [SPush v]
+ | AId i => [SLoad i]
+ | APlus a1 a2 => (s_compile a1) ++ (s_compile a2) ++ [SPlus]
+ | AMinus a1 a2 => (s_compile a1) ++ (s_compile a2) ++ [SMinus]
+ | AMult a1 a2 => (s_compile a1) ++ (s_compile a2) ++ [SMult]
+end.
 
 (** After you've defined [s_compile], prove the following to test
     that it works. *)
@@ -16,7 +22,7 @@ Example s_compile1 :
     s_compile (AMinus (AId X) (AMult (ANum 2) (AId Y)))
   = [SLoad X; SPush 2; SLoad Y; SMult; SMinus].
 Proof.
-  exact FILL_IN_HERE.
+reflexivity.
 Qed.
 
 (** **** Exercise: 3 stars, advanced (stack_compiler_correct)  *)
@@ -36,7 +42,19 @@ Qed.
 Theorem s_compile_correct : forall (st : state) (e : aexp),
   s_execute st [] (s_compile e) = [ aeval st e ].
 Proof.
-  exact FILL_IN_HERE.
+assert (K: forall (e : aexp) (st : state) (s1 : list nat) (other : list sinstr),
+    s_execute st s1 (s_compile e ++ other) =
+    s_execute st ((aeval st e) :: s1) other).
+{induction e; try reflexivity. simpl. intros. assert ((s_compile e1 ++ s_compile e2 ++ [SPlus]) ++ other = s_compile e1 ++ s_compile e2 ++ [SPlus] ++ other). rewrite app_ass. rewrite app_ass. reflexivity.
+  rewrite H. assert (s_execute st s1 (s_compile e1 ++ s_compile e2 ++ SPlus :: other) = s_execute st (aeval st e1 :: s1) (s_compile e2 ++ SPlus :: other)). apply IHe1. simpl. rewrite H0.
+  assert (s_execute st (aeval st e1 :: s1) (s_compile e2 ++ SPlus :: other) = s_execute st (aeval st e2 :: aeval st e1 :: s1) (SPlus :: other)). apply IHe2. rewrite H1. simpl. reflexivity.
+intros. assert (s_execute st s1 (s_compile e1 ++ s_compile e2 ++ SMinus :: other) = s_execute st (aeval st e1 :: s1) (s_compile e2 ++ SMinus :: other)). apply IHe1. assert ((s_compile e1 ++ s_compile e2 ++ [SMinus]) ++ other = s_compile e1 ++ s_compile e2 ++ [SMinus] ++ other). rewrite app_ass. rewrite app_ass. reflexivity.
+simpl. rewrite H0. simpl. rewrite H. assert (s_execute st (aeval st e1 :: s1) (s_compile e2 ++ SMinus :: other) = s_execute st (aeval st e2 :: aeval st e1 :: s1) (SMinus :: other)). apply IHe2. rewrite H1. simpl. reflexivity.
+  intros. assert ((s_compile e1 ++ s_compile e2 ++ [SMult]) ++ other = s_compile e1 ++ s_compile e2 ++ [SMult] ++ other). rewrite app_ass. rewrite app_ass. reflexivity.
+assert (s_execute st s1 (s_compile e1 ++ s_compile e2 ++ SMult :: other) = s_execute st (aeval st e1 :: s1) (s_compile e2 ++ SMult :: other)). apply IHe1. assert (s_execute st (aeval st e1 :: s1) (s_compile e2 ++ SMult :: other) = s_execute st (aeval st e2 :: aeval st e1 :: s1) (SMult :: other)).
+apply IHe2.  simpl. rewrite H. simpl. rewrite H0. simpl. rewrite H1. simpl. reflexivity. }
+intros. replace ([aeval st e]) with (s_execute st [aeval st e] []). replace (s_compile e) with (s_compile e++[]). apply K. 
+rewrite app_nil_end. reflexivity. reflexivity.
 Qed.
 
 (*-- Check --*)
