sf/Assignment08_01.v
@@ -7,7 +7,8 @@ Example ceval_example2:
     (X ::= ANum 0;; Y ::= ANum 1;; Z ::= ANum 2) / empty_state ||
     (update (update (update empty_state X 0) Y 1) Z 2).
 Proof.
-  exact FILL_IN_HERE.
+repeat eapply E_Seq; eapply E_Ass; simpl; exists.
+
 Qed.
 
 (*-- Check --*)
