sf/Assignment08_04.v
@@ -13,9 +13,15 @@ Theorem no_whiles_terminate: forall c st
     (NOWHL: no_whiles c = true),
   exists st', c / st || st'.
 Proof.
-  exact FILL_IN_HERE.
+intros. generalize dependent st. induction c.
+intros. exists st. constructor.
+intros st. exists (update st i (aeval st a)). constructor. reflexivity.
+intros. inversion NOWHL. assert (H1:= H0). apply andb_true_elim1 in H0. apply IHc1 with st in H0. inversion H0. apply andb_true_elim2 in H1. apply IHc2 with x in H1. inversion H1. exists x0. apply E_Seq with x. apply H. apply H2.
+intros. inversion NOWHL. assert (H1:=H0). apply andb_true_elim1 in H0. apply andb_true_elim2 in H1. apply IHc1 with st in H0. apply IHc2 with st in H1. inversion H0. inversion H1.
+remember (beval st b) as eval_b. destruct eval_b.
+exists x. apply E_IfTrue. rewrite Heqeval_b. reflexivity. apply H. exists x0. apply E_IfFalse. rewrite Heqeval_b. reflexivity. apply H2.
+intros. inversion NOWHL.
 Qed.
-
 (*-- Check --*)
 Check no_whiles_terminate: forall c st
     (NOWHL: no_whiles c = true),
