sf/Assignment08_06.v
@@ -10,8 +10,10 @@ Theorem skip_right: forall c,
   cequiv 
     (c;; SKIP) 
     c.
-Proof. 
-  exact FILL_IN_HERE.
+Proof.
+intros. unfold cequiv. intros. split.
+{ intros. inversion H. inversion H5. subst. apply H2. }
+{ intros. apply E_Seq with st'. apply H. apply E_Skip. }
 Qed.
 
 (*-- Check --*)
