sf/Assignment08_09.v
@@ -11,8 +11,18 @@ Theorem WHILE_true: forall b c,
      cequiv 
        (WHILE b DO c END)
        (WHILE BTrue DO SKIP END).
-Proof. 
-  exact FILL_IN_HERE.
+Proof.
+assert (WHILE_true_nonterm : forall b c st st', bequiv b BTrue -> ~( (WHILE b DO c END) / st || st' )).
+{ intros. unfold not. intros. remember (WHILE b DO c END) as cw. ceval_cases (induction H0) Case; inversion Heqcw; subst; clear Heqcw.
+  unfold bequiv in H. rewrite H in H0. inversion H0. apply IHceval2. reflexivity. }
+  intros. split; intros.
+  apply WHILE_true_nonterm in H0; [apply ex_falso_quodlibet; assumption | assumption].
+  apply WHILE_true_nonterm in H0.
+  apply ex_falso_quodlibet.
+  assumption.
+  unfold bequiv.
+  simpl.
+  reflexivity.
 Qed.
 
 (*-- Check --*)
