sf/Assignment08_11.v
@@ -7,7 +7,13 @@ Theorem assign_aequiv : forall X e,
   aequiv (AId X) e -> 
   cequiv SKIP (X ::= e).
 Proof.
-  exact FILL_IN_HERE.
+assert (K: forall n1 x1 x2 (st : state), st x1 = n1 -> (update st x1 n1) x2 = st x2).
+  { intros. inversion H. unfold update. remember (eq_id_dec x1 x2). destruct s. rewrite e. reflexivity. reflexivity. }
+intros. split.
+{ intros. inversion H0. subst. assert (st' = (update st' X (st' X))). apply functional_extensionality. intro. rewrite K. reflexivity. reflexivity.
+  rewrite H1. rewrite <- H1 in |-* at 1. apply E_Ass. rewrite <- H. simpl. reflexivity. }
+{ intros. inversion H0. subst. assert (st = update st X (aeval st e)). rewrite <- H. apply functional_extensionality. intros. rewrite K. reflexivity. simpl. reflexivity.
+  rewrite <- H1. constructor. }
 Qed.
 
 (*-- Check --*)
