sf/Assignment08_12.v
@@ -6,8 +6,10 @@ Require Export Assignment08_11.
 Theorem CSeq_congruence : forall c1 c1' c2 c2',
   cequiv c1 c1' -> cequiv c2 c2' ->
   cequiv (c1;;c2) (c1';;c2').
-Proof. 
-  exact FILL_IN_HERE.
+Proof.
+intros c1 c1' c2 c2' H1 H2. split.
+{ intro H3. inversion H3. subst. apply E_Seq with st'0. apply H1. apply H4. apply H2. apply H7. }
+{ intros H3. inversion H3. subst. apply E_Seq with st'0. apply H1. apply H4. apply H2. apply H7. }
 Qed.
 
 (*-- Check --*)
