sf/Assignment08_13.v
@@ -7,7 +7,10 @@ Theorem CIf_congruence : forall b b' c1 c1' c2 c2',
   bequiv b b' -> cequiv c1 c1' -> cequiv c2 c2' ->
   cequiv (IFB b THEN c1 ELSE c2 FI) (IFB b' THEN c1' ELSE c2' FI).
 Proof.
-  exact FILL_IN_HERE.
+intros. split.
+{ intros. inversion H2. subst. apply E_IfTrue. unfold bequiv in H. rewrite <- H8. rewrite H. reflexivity. apply H0. apply H9. subst.
+  apply E_IfFalse. rewrite <- H8. rewrite H. reflexivity. apply H1. apply H9. }
+{ intros. inversion H2. subst. apply E_IfTrue. rewrite <- H8. apply H. apply H0. apply H9. subst. apply E_IfFalse. rewrite <- H8. rewrite H. reflexivity. apply  H1. apply H9. }
 Qed.
 
 (*-- Check --*)
