sf/Assignment08_14.v
@@ -99,8 +99,11 @@ Proof.
       (* The only interesting case is when both a1 and a2 
          become constants after folding *)
       simpl. destruct (beq_nat n n0); reflexivity.
-  Case "BLe". 
-    exact FILL_IN_HERE.
+  Case "BLe".
+    simpl. remember (fold_constants_aexp a) as a'. remember (fold_constants_aexp a0) as a0'.
+    replace (aeval st a) with (aeval st a') by (subst a'; rewrite <- fold_constants_aexp_sound; reflexivity).
+    replace (aeval st a0) with (aeval st a0') by (subst a0'; rewrite <- fold_constants_aexp_sound; reflexivity).
+    destruct a';destruct a0';try reflexivity. simpl. destruct (ble_nat n n0). reflexivity. reflexivity.
   Case "BNot". 
     simpl. remember (fold_constants_bexp b) as b' eqn:Heqb'. 
     rewrite IHb.
