sf/Assignment08_16.v
@@ -5,9 +5,21 @@ Require Export Assignment08_15.
 Lemma optimize_0plus_aexp_sound:
   atrans_sound optimize_0plus_aexp.
 Proof.
-  exact FILL_IN_HERE.
+unfold atrans_sound. intros. unfold aequiv. intros.
+aexp_cases (induction a) Case; simpl.
+reflexivity.
+reflexivity.
+{ rewrite IHa1. rewrite IHa2. generalize dependent a2. destruct a1. destruct n. intros. simpl. reflexivity.
+  { destruct a2. simpl. destruct n0. simpl. intro.  rewrite plus_comm. reflexivity. simpl. reflexivity.
+    simpl. reflexivity. reflexivity. reflexivity. reflexivity. }
+  { destruct a2. simpl. destruct n. simpl. rewrite plus_comm. reflexivity. simpl. reflexivity. reflexivity. reflexivity. reflexivity. reflexivity. }
+  { destruct a2. intros. destruct n. simpl in IHa2. rewrite plus_comm. reflexivity. reflexivity. reflexivity. reflexivity. reflexivity. reflexivity. }
+  { destruct a2. destruct n. simpl. rewrite plus_comm. reflexivity. reflexivity. reflexivity. reflexivity. reflexivity. reflexivity. }
+  { destruct a2. destruct n. simpl. rewrite plus_comm. reflexivity. reflexivity. reflexivity. reflexivity. reflexivity. reflexivity. }
+}
+rewrite IHa1. rewrite IHa2. reflexivity.
+rewrite IHa1. rewrite IHa2. reflexivity.
 Qed.
-
 (*-- Check --*)
 Check optimize_0plus_aexp_sound:
   atrans_sound optimize_0plus_aexp.
