sf/Assignment08_17.v
@@ -5,7 +5,13 @@ Require Export Assignment08_16.
 Lemma optimize_0plus_bexp_sound:
   btrans_sound optimize_0plus_bexp.
 Proof.
-  exact FILL_IN_HERE.
+unfold btrans_sound. intros. unfold bequiv. intros.
+bexp_cases (induction b) Case. reflexivity. reflexivity.
+ assert (aeval st a = aeval st (optimize_0plus_aexp a)) as Ha1. apply optimize_0plus_aexp_sound. assert (aeval st a0 = aeval st (optimize_0plus_aexp a0)) as Ha2.
+ apply optimize_0plus_aexp_sound. simpl. rewrite -> Ha1. rewrite -> Ha2. reflexivity.
+simpl. assert (aeval st a = aeval st (optimize_0plus_aexp a)) as Ha1. apply optimize_0plus_aexp_sound. assert (aeval st a0 = aeval st (optimize_0plus_aexp a0)) as Ha2.
+apply optimize_0plus_aexp_sound. rewrite -> Ha1. rewrite -> Ha2. reflexivity.
+simpl. rewrite <- IHb. reflexivity. simpl. rewrite <- IHb1. rewrite <- IHb2. reflexivity.
 Qed.
 
 (*-- Check --*)
