sf/Assignment08_19.v
@@ -5,7 +5,8 @@ Require Export Assignment08_18.
 Lemma constfold_0plus_sound:
   ctrans_sound constfold_0plus.
 Proof.
-  exact FILL_IN_HERE.
+unfold constfold_0plus. unfold ctrans_sound. intros. remember (fold_constants_com c) as c'. apply trans_cequiv with c'.
+rewrite Heqc'. apply fold_constants_com_sound. apply optimize_0plus_com_sound.
 Qed.
 
 (*-- Check --*)
